Hs/HsTerm.lean
@@ -1,2 +1,3 @@
 import Hs.HsTerm.Definition
 import Hs.HsTerm.Substitution
+import Hs.HsTerm.Lemmas
