Hs/Monad.lean
@@ -1,0 +1,27 @@
+
+
+abbrev DsM a := Except Std.Format a
+
+namespace DsM
+
+def ok : a -> DsM a := λ x => Except.ok x
+def error : Std.Format -> DsM a := λ x => Except.error x
+def bind : DsM a -> (a -> DsM b) -> DsM b := Except.bind
+
+def toDsM (pfix : Std.Format) : Option a -> DsM a
+| .some a => ok a
+| .none => error (pfix ++ Std.Format.line)
+
+def toDsMq : Option a -> DsM a := toDsM ""
+
+def run [Repr a] : DsM a -> Std.Format
+| .error e => "Error:" ++ Std.Format.line ++ e
+| .ok t => repr t
+
+end DsM
+
+instance beq_DsMa [BEq a] : BEq (DsM a) where
+     beq x y :=
+       match (x, y) with
+       | (.ok x, .ok y) => x == y
+       | _ => False
