SystemFD/Term.lean
@@ -5,3 +5,4 @@ import SystemFD.Term.Substitution
 import SystemFD.Term.Instances
 import SystemFD.Term.Subexpression
 import SystemFD.Term.Shape
+import SystemFD.Term.Lemmas
