SystemFD/Term/Lemmas.lean
@@ -1,0 +1,37 @@
+import SystemFD.Term.Equality
+import SystemFD.Term.Definition
+import SystemFD.Term.Substitution
+import SystemFD.Term.Shape
+
+namespace Term
+
+theorem application_spine_size (τ : Term) :
+  τ.neutral_form = .some nf ->
+  ∀ τ' : Term, (nf.2.map (·.2)).elem τ' ->
+  τ'.size < τ.size := by
+  intro h1 τ' h2
+  simp_all; cases h2;
+  case _ h2 =>
+  induction τ generalizing nf τ';
+  any_goals (simp at h1)
+  case _ =>
+    cases h1; case _ h1 h3 =>
+    simp at h2;
+  case _ v _ _ ih1 ih2 =>
+    cases v <;> simp at h1
+    all_goals(
+      rw[Option.bind_eq_some] at h1; cases h1;
+      case _ sp' nf =>
+      cases nf; case _ anf nf =>
+      cases nf; simp at h2;
+      cases h2;
+      case _ h2 =>
+        replace ih1 := ih1 anf τ' h2
+        simp; omega;
+      case _ h2 =>
+        cases h2; case _ r l =>
+        replace ih1 := ih1 anf τ'
+        cases l; cases r; simp; omega;
+    )
+
+end Term
